examples/Isa.v
@@ -14,7 +14,8 @@ Require Import Ex.MemTypes Ex.SC.
  * Just one RV32M instruction: MUL
  *)
 Section RV32I.
-  Definition rv32iAddrSize := 5. (* 2^5 = 32 memory cells *)
+  Definition rv32iAddrSize := 7. (* 2^7 memory cells *)
+  Definition rv32iIAddrSize := 5. (* 2^5 = 32 program size *)
   Definition rv32iLgDataBytes := 4. (* TODO: invalid name; DataBytes is right *)
   Definition rv32iOpIdx := 7. (* always inst[6-0] *)
   Definition rv32iRfIdx := 5. (* 2^5 = 32 general purpose registers, x0 is hardcoded though *)
@@ -272,9 +273,9 @@ Section RV32I.
       exact ($$Default)%kami_expr.
   Defined.
 
-  Definition rv32iAlignPc: AlignPcT rv32iAddrSize.
+  Definition rv32iAlignPc: AlignPcT rv32iAddrSize rv32iIAddrSize.
     unfold AlignPcT; intros ty pc.
-    exact (#pc >> $$(natToWord 2 2))%kami_expr.
+    exact (UniBit (ZeroExtendTrunc _ _) (#pc >> $$(natToWord 2 2)))%kami_expr.
   Defined.
 
   (* NOTE: Because instructions are not on the memory, we give (pc + 1) for the next pc.
