examples/ProcDecSCN.v
@@ -11,7 +11,7 @@ Require Import Ex.ProcDec Ex.ProcDecInl Ex.ProcDecInv Ex.ProcDecSC.
 Set Implicit Arguments.
 
 Section ProcDecSCN.
-  Variables addrSize fifoSize lgDataBytes rfIdx: nat.
+  Variables addrSize iaddrSize fifoSize lgDataBytes rfIdx: nat.
 
   (* External abstract ISA: decoding and execution *)
   Variables (getOptype: OptypeT lgDataBytes)
@@ -28,7 +28,7 @@ Section ProcDecSCN.
             (getDst: DstT lgDataBytes rfIdx)
             (exec: ExecT addrSize lgDataBytes)
             (getNextPc: NextPcT addrSize lgDataBytes rfIdx)
-            (alignPc: AlignPcT addrSize).
+            (alignPc: AlignPcT addrSize iaddrSize).
 
   Variable n: nat.
   
