examples/ProcFDCorrect.v
@@ -11,7 +11,7 @@ Require Import Eqdep.
 Set Implicit Arguments.
 
 Section FetchDecode.
-  Variables addrSize lgDataBytes rfIdx: nat.
+  Variables addrSize iaddrSize lgDataBytes rfIdx: nat.
 
   (* External abstract ISA: decoding and execution *)
   Variables (getOptype: OptypeT lgDataBytes)
@@ -28,7 +28,7 @@ Section FetchDecode.
             (getDst: DstT lgDataBytes rfIdx)
             (exec: ExecT addrSize lgDataBytes)
             (getNextPc: NextPcT addrSize lgDataBytes rfIdx)
-            (alignPc: AlignPcT addrSize)
+            (alignPc: AlignPcT addrSize iaddrSize)
             (predictNextPc: forall ty, fullType ty (SyntaxKind (Bit addrSize)) -> (* pc *)
                                        Expr ty (SyntaxKind (Bit addrSize))).
 
@@ -101,7 +101,7 @@ Section FetchDecode.
 
   Definition fetchDecode_regMap (r: RegsT): RegsT :=
     (mlet pcv : (Bit addrSize) <- r |> "pc";
-       mlet pgmv : (Vector (Data lgDataBytes) addrSize) <- r |> "pgm";
+       mlet pgmv : (Vector (Data lgDataBytes) iaddrSize) <- r |> "pgm";
        mlet fev : Bool <- r |> "fEpoch";
        mlet f2dfullv : Bool <- r |> "f2d"--"full";
        mlet f2deltv : f2dElt <- r |> "f2d"--"elt";
