examples/ProcFDInl.v
@@ -5,7 +5,7 @@ Require Import Ex.SC Ex.MemTypes Ex.ProcFetchDecode.
 Set Implicit Arguments.
 
 Section Inlined.
-  Variables addrSize lgDataBytes rfIdx: nat.
+  Variables addrSize iaddrSize lgDataBytes rfIdx: nat.
 
   (* External abstract ISA: decoding and execution *)
   Variables (getOptype: OptypeT lgDataBytes)
@@ -22,7 +22,7 @@ Section Inlined.
             (getDst: DstT lgDataBytes rfIdx)
             (exec: ExecT addrSize lgDataBytes)
             (getNextPc: NextPcT addrSize lgDataBytes rfIdx)
-            (alignPc: AlignPcT addrSize)
+            (alignPc: AlignPcT addrSize iaddrSize)
             (predictNextPc: forall ty, fullType ty (SyntaxKind (Bit addrSize)) -> (* pc *)
                                        Expr ty (SyntaxKind (Bit addrSize))).
 
