examples/ProcThreeStDec.v
@@ -11,7 +11,7 @@ Require Import Eqdep.
 Set Implicit Arguments.
 
 Section ProcThreeStDec.
-  Variables addrSize lgDataBytes rfIdx: nat.
+  Variables addrSize iaddrSize lgDataBytes rfIdx: nat.
 
   (* External abstract ISA: decoding and execution *)
   Variables (getOptype: OptypeT lgDataBytes)
@@ -28,7 +28,7 @@ Section ProcThreeStDec.
             (getDst: DstT lgDataBytes rfIdx)
             (exec: ExecT addrSize lgDataBytes)
             (getNextPc: NextPcT addrSize lgDataBytes rfIdx)
-            (alignPc: AlignPcT addrSize)
+            (alignPc: AlignPcT addrSize iaddrSize)
             (predictNextPc: forall ty, fullType ty (SyntaxKind (Bit addrSize)) -> (* pc *)
                                        Expr ty (SyntaxKind (Bit addrSize))).
 
@@ -130,7 +130,7 @@ Section ProcThreeStDec.
 
   Definition p3st_pdec_regMap (r: RegsT): RegsT :=
     (mlet pcv : (Bit addrSize) <- r |> "pc";
-       mlet pgmv : (Vector (Data lgDataBytes) addrSize) <- r |> "pgm";
+       mlet pgmv : (Vector (Data lgDataBytes) iaddrSize) <- r |> "pgm";
        mlet rfv : (Vector (Data lgDataBytes) rfIdx) <- r |> "rf";
        mlet d2eeltv : d2eElt <- r |> "d2e"--"elt";
        mlet d2efv : Bool <- r |> "d2e"--"full";
