examples/ProcThreeStInv.v
@@ -10,7 +10,7 @@ Require Import Eqdep ProofIrrelevance.
 Set Implicit Arguments.
 
 Section Invariants.
-  Variables addrSize lgDataBytes rfIdx: nat.
+  Variables addrSize iaddrSize lgDataBytes rfIdx: nat.
 
   (* External abstract ISA: decoding and execution *)
   Variables (getOptype: OptypeT lgDataBytes)
@@ -27,7 +27,7 @@ Section Invariants.
             (getDst: DstT lgDataBytes rfIdx)
             (exec: ExecT addrSize lgDataBytes)
             (getNextPc: NextPcT addrSize lgDataBytes rfIdx)
-            (alignPc: AlignPcT addrSize)
+            (alignPc: AlignPcT addrSize iaddrSize)
             (predictNextPc: forall ty, fullType ty (SyntaxKind (Bit addrSize)) -> (* pc *)
                                        Expr ty (SyntaxKind (Bit addrSize))).
 
@@ -210,7 +210,7 @@ Section Invariants.
 
   (* NOTE: this invariant requires p3st_raw_inv *)
   Definition p3st_decode_inv_body
-             (pgmv: fullType type (SyntaxKind (Vector (Data lgDataBytes) addrSize)))
+             (pgmv: fullType type (SyntaxKind (Vector (Data lgDataBytes) iaddrSize)))
              (rfv: fullType type (SyntaxKind (Vector (Data lgDataBytes) rfIdx)))
              (d2eeltv: fullType type (SyntaxKind d2eElt))
              (d2efullv: fullType type (SyntaxKind Bool)) :=
@@ -236,7 +236,7 @@ Section Invariants.
       evalExpr (d2eVal2 _ d2eeltv) = rfv (evalExpr (getSrc2 _ rawInst)))).
 
   Record p3st_decode_inv (o: RegsT) : Prop :=
-    { pgmv2 : fullType type (SyntaxKind (Vector (Data lgDataBytes) addrSize));
+    { pgmv2 : fullType type (SyntaxKind (Vector (Data lgDataBytes) iaddrSize));
       Hpgmv2 : M.find "pgm"%string o = Some (existT _ _ pgmv2);
 
       rfv2 : fullType type (SyntaxKind (Vector (Data lgDataBytes) rfIdx));
@@ -258,7 +258,7 @@ Section Invariants.
 
   (* NOTE: this invariant requires p3st_decode_inv *)
   Definition p3st_stalled_inv_body
-             (pgmv: fullType type (SyntaxKind (Vector (Data lgDataBytes) addrSize)))
+             (pgmv: fullType type (SyntaxKind (Vector (Data lgDataBytes) iaddrSize)))
              (rfv: fullType type (SyntaxKind (Vector (Data lgDataBytes) rfIdx)))
              (stallv: fullType type (SyntaxKind Bool))
              (stalledv: fullType type (SyntaxKind d2eElt)) :=
@@ -270,7 +270,7 @@ Section Invariants.
      evalExpr (d2eDst _ stalledv) = evalExpr (getLdDst _ rawInst)).
 
   Record p3st_stalled_inv (o: RegsT) : Prop :=
-    { pgmv3 : fullType type (SyntaxKind (Vector (Data lgDataBytes) addrSize));
+    { pgmv3 : fullType type (SyntaxKind (Vector (Data lgDataBytes) iaddrSize));
       Hpgmv3 : M.find "pgm"%string o = Some (existT _ _ pgmv3);
 
       rfv3 : fullType type (SyntaxKind (Vector (Data lgDataBytes) rfIdx));
